Demo.v
@@ -1,3 +1,4 @@
+Require Import SGA.Types.
 Require Import SGA.Notations.
 
 Require Import Coq.Strings.String.
@@ -6,21 +7,26 @@ Open Scope string_scope.
 Record demo_package_t :=
   { dp_var_t : Type;
     dp_reg_t : Type;
-    dp_name_t : Type;
-    dp_custom_fn_t : Type;
-    sga : @sga_package_t dp_var_t dp_reg_t dp_name_t dp_custom_fn_t;
-    vp : @verilog_package_t dp_var_t dp_reg_t dp_name_t dp_custom_fn_t;
-    sp : @sim_package_t dp_var_t dp_reg_t dp_name_t dp_custom_fn_t }.
+    dp_rule_name_t : Type;
+    dp_ext_fn_t : Type;
+    sga : @sga_package_t dp_var_t dp_reg_t dp_rule_name_t dp_ext_fn_t;
+    vp : @verilog_package_t dp_var_t dp_reg_t dp_rule_name_t dp_ext_fn_t;
+    sp : @sim_package_t dp_var_t dp_reg_t dp_rule_name_t dp_ext_fn_t }.
 
 Notation opt := simplify_bool_1.
-Notation interop_opt := (lco_opt_compose simplify_bool_1 elaborate_externals_1).
-Notation uaction := (uaction unit string).
+Notation interop_opt := simplify_bool_1.
+
+Definition pos_t := unit.
+Definition var_t := string.
+Definition fn_name_t := string.
+Notation uaction := (uaction pos_t var_t fn_name_t).
+Notation UInternalFunction reg_t ext_fn_t := (InternalFunction fn_name_t var_t (uaction reg_t ext_fn_t)).
 
 Module Ex1.
   Notation var_t := string.
   Inductive reg_t := R0 | R1.
   Inductive fn_t := Even | Odd.
-  Inductive name_t := r1.
+  Inductive rule_name_t := r1.
 
   Definition R reg : type :=
     match reg with
@@ -30,11 +36,10 @@ Module Ex1.
 
   Definition Sigma fn : ExternalSignature :=
     match fn with
-    | Even => {{ bits_t 3 ~> unit_t ~> bits_t 1}}
-    | Odd => {{ bits_t 3 ~> unit_t ~> bits_t 1}}
+    | Even => {{ bits_t 3 ~> bits_t 1}}
+    | Odd => {{ bits_t 3 ~> bits_t 1}}
     end.
 
-  Definition uSigma (fn: fn_t) (_ _: type) : result fn_t fn_tc_error := Success fn.
 
   Definition r idx : R idx :=
     match idx with
@@ -42,44 +47,42 @@ Module Ex1.
     | R1 => Ob~0
     end.
 
-  Definition sigma idx : Sigma idx :=
+  Definition sigma idx : Sig_denote (Sigma idx) :=
     match idx with
-    | Even => fun (bs: bits 3) _ => Ob~(negb (Bits.lsb bs))
-    | Odd => fun (bs: bits 3) _ => Ob~(Bits.lsb bs)
+    | Even => fun (bs: bits 3) => Ob~(negb (Bits.lsb bs))
+    | Odd => fun (bs: bits 3) => Ob~(Bits.lsb bs)
     end.
 
-  Example uactions r : uaction var_t reg_t (interop_ufn_t fn_t) :=
+  Example uactions r : uaction reg_t fn_t :=
     match r with
     | r1 =>
       {$ let "x" := read0(R0) in
-         if (`UCall (UCustomFn Even) (UVar "x") (UConstBits Ob)`)
+         if (`UExternalCall Even (UVar "x")`)
          then write0(R1,`UConstBits Ob~1`)
          else write0(R1,`UConstBits Ob~1`)
                        $}
     end.
 
   Definition rules :=
-    tc_rules R (interop_Sigma Sigma) (interop_uSigma uSigma) uactions.
+    tc_rules R Sigma uactions.
 
-  Example us1 : uscheduler unit name_t :=
+  Example us1 : uscheduler unit rule_name_t :=
     UTry r1 UDone UDone.
 
   Definition s1 :=
     tc_scheduler us1.
 
   Definition s1_result :=
-    Eval compute in interp_scheduler (ContextEnv.(create) r) (interop_sigma sigma) rules s1.
+    Eval compute in interp_scheduler (ContextEnv.(create) r) sigma rules s1.
 
   Definition s1_circuit :=
-    compile_scheduler opt (ContextEnv.(create) (readRegisters R (interop_Sigma Sigma))) rules s1.
+    compile_scheduler opt (ContextEnv.(create) (readRegisters R Sigma)) rules s1.
 End Ex1.
 
 Module Ex2.
-  Definition var_t := string.
   Inductive reg_t := R0 | R1 | R2.
-  Inductive ufn_t := UOr | UNot.
-  Inductive fn_t := Or (n: nat) | Not (n: nat).
-  Inductive name_t := negate | swap_or_replace.
+  Definition fn_t := empty_ext_fn_t.
+  Inductive rule_name_t := negate | swap_or_replace.
 
   Definition R r :=
     match r with
@@ -88,26 +91,13 @@ Module Ex2.
     | R2 => bits_t 1
     end.
 
-  Definition Sigma fn :=
-    match fn with
-    | Or n => {{ bits_t n ~> bits_t n ~> bits_t n }}
-    | Not n => {{ bits_t n ~> unit_t ~> bits_t n }}
-    end.
-
-  Definition uSigma fn (tau1 _: type) :=
-    let/res sz1 := assert_bits_t Arg1 tau1 in
-    Success match fn with
-            | UOr => Or sz1
-            | UNot => Not sz1
-            end.
-
-  Example _negate : uaction var_t reg_t ufn_t  :=
+  Example _negate : uaction reg_t fn_t  :=
     {$
        let "x" := read1(R0) in
        write1(R0,"x")
                 $}.
 
-  Example _swap_or_replace : uaction var_t reg_t ufn_t  :=
+  Example _swap_or_replace : uaction reg_t fn_t  :=
     {$
       let "should_swap" := read0(R2) in
       if "should_swap"
@@ -115,24 +105,23 @@ Module Ex2.
         write0(R1,read0(R0));
         write0(R0,read0(R1))
       else
-        write0(R0,`UCall (UCustomFn UOr) {$ read0(R0) $} {$  read0(R1) $} `)
+        write0(R0, read0(R0) || read0(R1))
                  $}.
 
-
-  Example _ill_typed_write : uaction var_t reg_t ufn_t  :=
+  Example _ill_typed_write : uaction reg_t fn_t  :=
     UWrite P0 R2 (URead P0 R1).
 
-  Example _unbound_variable : uaction var_t reg_t ufn_t  :=
+  Example _unbound_variable : uaction reg_t fn_t  :=
     UWrite P0 R0 (UVar "y").
 
-  Example tsched : scheduler name_t :=
+  Example tsched : scheduler rule_name_t :=
     tc_scheduler (UTry swap_or_replace (UTry negate UDone UDone) (UTry negate UDone UDone)).
 
   Fail Example trule : rule var_t R Sigma :=
-    tc_rule R Sigma uSigma _ill_typed_write.
+    tc_rule R Sigma _ill_typed_write.
 
   Fail Example trule : rule var_t R Sigma :=
-    tc_rule R Sigma uSigma _unbound_variable.
+    tc_rule R Sigma _unbound_variable.
 
   Definition r idx : R idx :=
     match idx with
@@ -141,23 +130,17 @@ Module Ex2.
     | R2 => Ob~1
     end.
 
-  Definition sigma idx : Sigma idx :=
-    match idx with
-    | Or n => fun bs1 bs2 => Bits.map2 orb bs1 bs2
-    | Not n => fun bs _ => Bits.map negb bs
-    end.
-
-  Definition rules : name_t -> rule var_t R (interop_Sigma Sigma) :=
-    tc_rules R (interop_Sigma Sigma) (interop_uSigma uSigma)
+  Definition rules : rule_name_t -> rule var_t R empty_Sigma :=
+    tc_rules R empty_Sigma
              (fun r => match r with
                     | negate => _negate
                     | swap_or_replace => _swap_or_replace
                     end).
 
   Definition tsched_result :=
-    Eval compute in interp_scheduler (ContextEnv.(create) r) (interop_sigma sigma) rules tsched.
+    Eval compute in interp_scheduler (ContextEnv.(create) r) empty_sigma rules tsched.
   Definition tsched_circuit :=
-    compile_scheduler opt (ContextEnv.(create) (readRegisters R (interop_Sigma Sigma))) rules tsched.
+    compile_scheduler opt (ContextEnv.(create) (readRegisters R empty_Sigma)) rules tsched.
 End Ex2.
 
 Notation compute t :=
@@ -166,10 +149,9 @@ Notation compute t :=
         exact (t: tt)) (only parsing).
 
 Module Collatz.
-  Definition var_t := string.
   Inductive reg_t := R0.
-  Definition ufn_t := interop_minimal_ufn_t.
-  Inductive name_t := divide | multiply.
+  Definition fn_t := empty_ext_fn_t.
+  Inductive rule_name_t := divide | multiply.
 
   Definition logsz := 4.
   Notation sz := (pow2 logsz).
@@ -183,16 +165,15 @@ Module Collatz.
     match idx with
     | R0 => Bits.of_nat 16 19
     end.
-  Notation uaction := (uaction var_t reg_t ufn_t).
-  Notation InternalFunction := (UInternalFunction unit string reg_t ufn_t).
+
   Notation zero := (Bits.zero logsz).
   Notation one := (Bits.zero logsz).
 
-  Definition times_three  : InternalFunction :=
+  Definition times_three : UInternalFunction reg_t fn_t :=
     function "times_three" ("arg1" : bits_t 16) : bits_t 16 :=
      ("arg1" << #Ob~1)  + "arg1".
 
-  Definition _divide : uaction :=
+  Definition _divide : uaction reg_t fn_t :=
   {$
     let "v" := read0(R0) in
     let "odd" := "v"[#Ob~0~0~0~0] in
@@ -202,7 +183,7 @@ Module Collatz.
       fail
   $}.
 
-  Definition _multiply : uaction :=
+  Definition _multiply : uaction reg_t fn_t :=
   {$
     let "v" := read1(R0) in
     let "odd" := "v"[#Ob~0~0~0~0] in
@@ -219,32 +200,32 @@ Module Collatz.
 
   (* Typechecking  *)
   Definition rules :=
-    tc_rules R interop_minimal_Sigma interop_minimal_uSigma
+    tc_rules R empty_Sigma
              (fun r => match r with
                     | divide => _divide
                     | multiply => _multiply
                     end).
 
   Definition result :=
-    compute (interp_scheduler cr interop_minimal_sigma rules collatz).
+    compute (interp_scheduler cr empty_sigma rules collatz).
 
   Definition divide_result :=
-    compute (interp_action cr interop_minimal_sigma CtxEmpty log_empty log_empty
+    compute (interp_action cr empty_sigma CtxEmpty log_empty log_empty
                            (rules divide)).
 
   Definition multiply_result :=
-    compute (interp_action cr interop_minimal_sigma CtxEmpty log_empty log_empty
+    compute (interp_action cr empty_sigma CtxEmpty log_empty log_empty
                            (rules multiply)).
 
   Definition circuit :=
-    compile_scheduler interop_opt (ContextEnv.(create) (readRegisters R interop_minimal_Sigma)) rules collatz.
+    compile_scheduler interop_opt (ContextEnv.(create) (readRegisters R empty_Sigma)) rules collatz.
 
   Definition sga_package :=
     {| sga_reg_types := R;
        sga_reg_init := r;
        sga_reg_finite := _;
 
-       sga_custom_fn_types := interop_empty_Sigma;
+       sga_ext_fn_types := empty_Sigma;
 
        sga_reg_names r := match r with
                          | R0 => "r0"
@@ -263,26 +244,24 @@ Module Collatz.
     {| sga := sga_package;
        sp := {| sp_pkg := sga_package;
                sp_var_names x := x;
-               sp_custom_fn_names := interop_empty_fn_names;
+               sp_ext_fn_names := empty_fn_names;
                sp_extfuns := None |};
        vp := {| vp_pkg := sga_package;
                vp_external_rules := List.nil;
-               vp_custom_fn_names := interop_empty_fn_names |} |}.
-  Check package.
+               vp_ext_fn_names := empty_fn_names |} |}.
 End Collatz.
 
 Require Import Coq.Lists.List.
 
 Module Type Unpacker.
-  Axiom unpack : forall reg_t custom_ufn_t (source: string), uaction string reg_t (interop_ufn_t custom_ufn_t).
+  Axiom unpack : forall reg_t ext_fn_t (source: string), uaction reg_t ext_fn_t.
 End Unpacker.
 
 Module Type Fetcher.
-  Axiom custom_fn_t : Type.
-  Axiom custom_Sigma : custom_fn_t -> ExternalSignature.
-  Axiom custom_uSigma : custom_fn_t -> type -> type -> result custom_fn_t fn_tc_error.
-  Axiom custom_fn_names : custom_fn_t -> string.
-  Axiom fetch_instr : forall reg_t (pc: string), uaction string reg_t (interop_ufn_t custom_fn_t).
+  Axiom ext_fn_t : Type.
+  Axiom Sigma : ext_fn_t -> ExternalSignature.
+  Axiom ext_fn_names : ext_fn_t -> string.
+  Axiom fetch_instr : forall reg_t (pc: string), uaction reg_t ext_fn_t.
 End Fetcher.
 
 Definition decoded_sig :=
@@ -293,13 +272,11 @@ Definition decoded_sig :=
                        :: nil |}.
 
 Module Decoder (P: Unpacker) (F: Fetcher).
-  Definition var_t := string.
   Inductive reg_t := Rpc | Rencoded | Rdecoded.
-  Definition ufn_t := interop_ufn_t F.custom_fn_t.
-  Inductive name_t := fetch | decode.
+  Definition fn_t := F.ext_fn_t.
+  Inductive rule_name_t := fetch | decode.
 
-  Definition Sigma := interop_Sigma F.custom_Sigma.
-  Definition uSigma := interop_uSigma F.custom_uSigma.
+  Definition Sigma := F.Sigma.
 
   Definition logsz := 5.
   Notation sz := (pow2 logsz).
@@ -320,18 +297,15 @@ Module Decoder (P: Unpacker) (F: Fetcher).
     | Rdecoded => (zero, (zero, (zero, tt)))
     end.
 
-  Notation uaction := (uaction var_t reg_t ufn_t).
-
-  Definition _fetch : uaction :=
+  Definition _fetch : uaction reg_t fn_t :=
     {$
     let "pc" := read0(Rpc) in
     let "encoded" := `F.fetch_instr _ "pc"` in
     write0(Rencoded,"encoded");
     write0(Rpc,"pc" + `UConstBits Ob~0~0~1`)
-                $}
-  .
+                $}.
 
-  Definition _decode : uaction :=
+  Definition _decode : uaction reg_t fn_t :=
     {$
     let "encoded" := read1(Rencoded) in
     write0(Rdecoded,`P.unpack _ _ "encoded"`)
@@ -346,7 +320,7 @@ Module Decoder (P: Unpacker) (F: Fetcher).
   (*   __must_typecheck_cbn R Sigma tcres. *)
 
   Notation rulemap_t :=
-    (name_t -> rule string R (interop_Sigma F.custom_Sigma)).
+    (rule_name_t -> rule string R F.Sigma).
 
   Definition make_package (modname: string) (rules: rulemap_t) :=
     let sga_package :=
@@ -354,7 +328,7 @@ Module Decoder (P: Unpacker) (F: Fetcher).
            sga_reg_init := r;
            sga_reg_finite := _;
 
-           sga_custom_fn_types := F.custom_Sigma;
+           sga_ext_fn_types := F.Sigma;
 
            sga_reg_names r := match r with
                              | Rpc => "Rpc"
@@ -373,31 +347,30 @@ Module Decoder (P: Unpacker) (F: Fetcher).
     let sim :=
         {| sp_pkg := sga_package;
            sp_var_names := fun x => x;
-           sp_custom_fn_names := F.custom_fn_names;
+           sp_ext_fn_names := F.ext_fn_names;
 
            sp_extfuns := Some "#include ""../extfuns.hpp""
 using extfuns = decoder_extfuns;" |} in
     let verilog :=
         {| vp_pkg := sga_package;
            vp_external_rules := List.nil;
-           vp_custom_fn_names := F.custom_fn_names |} in
+           vp_ext_fn_names := F.ext_fn_names |} in
     {| sga := sga_package; sp := sim; vp := verilog |}.
 End Decoder.
 
 Module ManualUnpacker <: Unpacker.
-  Notation SCall fn a1 a2 :=
-    (UCall (UPrimFn (UStructFn fn)) a1 a2).
+  Notation SCall1 fn a1 := (UUnop (UStruct1 fn) a1).
+  Notation SCall2 fn a1 a2 := (UBinop (UStruct2 fn) a1 a2).
 
-  Definition unpack reg_t custom_ufn_t encoded: uaction string reg_t (interop_ufn_t custom_ufn_t) :=
+  Definition unpack reg_t ext_fn_t encoded: uaction reg_t ext_fn_t :=
     {$
-       let "imm" := `SCall (UDoBits decoded_sig GetField "immediate") {$ encoded $} (UConstBits Ob)` in
-       let "src" := `SCall (UDoBits decoded_sig GetField "src") {$ encoded $} (UConstBits Ob)` in
-       let "dst" := `SCall (UDoBits decoded_sig GetField "dst") {$ encoded $} (UConstBits Ob)` in
-       `SCall (UDo SubstField "immediate")
-               (SCall (UDo SubstField "dst")
-                      (SCall (UDo SubstField "src")
-                             (UCall (UPrimFn (UConvFn (UInit (struct_t decoded_sig))))
-                                    (UConstBits Ob) (UConstBits Ob))
+       let "imm" := `SCall1 (UGetFieldBits decoded_sig "immediate") {$ encoded $}` in
+       let "src" := `SCall1 (UGetFieldBits decoded_sig "src") {$ encoded $}` in
+       let "dst" := `SCall1 (UGetFieldBits decoded_sig "dst") {$ encoded $}` in
+       `SCall2 (USubstField "immediate")
+               (SCall2 (USubstField "dst")
+                      (SCall2 (USubstField "src")
+                             (UUnop (UConv (UUnpack (struct_t decoded_sig))) (UConstBits (Bits.zero 32)))
                              {$"src"$})
                      {$"dst"$})
                {$"imm"$}`
@@ -405,21 +378,18 @@ Module ManualUnpacker <: Unpacker.
 End ManualUnpacker.
 
 Module PrimitiveUnpacker <: Unpacker.
-  Definition unpack reg_t custom_ufn_t encoded: uaction string reg_t (interop_ufn_t custom_ufn_t) :=
-    (UCall (UPrimFn (UConvFn (UUnpack (struct_t decoded_sig))))
-           (UVar encoded) (UConstBits Ob)).
+  Definition unpack reg_t ext_fn_t encoded: uaction reg_t ext_fn_t :=
+    (UUnop (UConv (UUnpack (struct_t decoded_sig))) (UVar encoded)).
 End PrimitiveUnpacker.
 
 Module ManualFetcher <: Fetcher.
   Import ListNotations.
 
-  Definition var_t := string.
-  Definition custom_fn_t := interop_empty_t.
-  Definition custom_Sigma := interop_empty_Sigma.
-  Definition custom_uSigma := interop_empty_uSigma.
-  Definition custom_fn_names := interop_empty_fn_names.
+  Definition ext_fn_t := empty_ext_fn_t.
+  Definition Sigma := empty_Sigma.
+  Definition ext_fn_names := empty_fn_names.
 
-  Notation uaction reg_t := (uaction string reg_t (interop_ufn_t custom_fn_t)).
+  Notation uaction reg_t := (uaction reg_t ext_fn_t).
 
   Definition instructions {reg_t} : list (uaction reg_t) :=
     List.map USugar
@@ -447,26 +417,23 @@ Module ManualFetcher <: Fetcher.
 End ManualFetcher.
 
 Module PrimitiveFetcher <: Fetcher.
-  Definition var_t := string.
-  Inductive custom_fn_t' := FetchInstr.
-  Definition custom_fn_t := custom_fn_t'.
+  Inductive ext_fn_t' := FetchInstr.
+  Definition ext_fn_t := ext_fn_t'.
 
-  Definition custom_Sigma (fn: custom_fn_t) : ExternalSignature :=
+  Definition Sigma (fn: ext_fn_t) : ExternalSignature :=
     match fn with
-    | FetchInstr => {{ bits_t 3 ~> unit_t ~> bits_t 32 }}
+    | FetchInstr => {{ bits_t 3 ~> bits_t 32 }}
     end.
 
-  Definition custom_uSigma (fn: custom_fn_t) (_ _: type) : result custom_fn_t fn_tc_error := Success fn.
-
-  Definition custom_fn_names (fn: custom_fn_t) : string :=
+  Definition ext_fn_names (fn: ext_fn_t) : string :=
     match fn with
     | FetchInstr => "fetch_instr"
     end.
 
-  Notation uaction reg_t := (uaction string reg_t (interop_ufn_t custom_fn_t)).
+  Notation uaction reg_t := (uaction reg_t ext_fn_t).
 
   Definition fetch_instr reg_t pc : uaction reg_t :=
-    Eval compute in (UCall (UCustomFn FetchInstr) (UVar pc) (UConstBits Ob)).
+    Eval compute in (UExternalCall FetchInstr (UVar pc)).
 End PrimitiveFetcher.
 
 Module ManualDecoder.
@@ -474,7 +441,7 @@ Module ManualDecoder.
   Include (Decoder ManualUnpacker F).
 
   Definition rules :=
-    tc_rules R Sigma uSigma
+    tc_rules R Sigma
              (fun r => match r with
                     | fetch => _fetch
                     | decode => _decode
@@ -491,7 +458,7 @@ Module PrimitiveDecoder.
   Include (Decoder PrimitiveUnpacker F).
 
   Definition rules :=
-    tc_rules R (interop_Sigma F.custom_Sigma) (interop_uSigma F.custom_uSigma)
+    tc_rules R F.Sigma
              (fun r => match r with
                     | fetch => _fetch
                     | decode => _decode
@@ -504,11 +471,10 @@ Module PrimitiveDecoder.
 End PrimitiveDecoder.
 
 Module Pipeline.
-  Definition var_t := string.
   Inductive reg_t := r0 | outputReg | inputReg | invalid | correct.
-  Inductive custom_fn_t := Stream | F | G.
-  Definition ufn_t := interop_ufn_t custom_fn_t.
-  Inductive name_t := doF | doG.
+  Inductive ext_fn_t := Stream | F | G.
+  Definition fn_t := ext_fn_t.
+  Inductive rule_name_t := doF | doG.
 
   Definition sz := (pow2 5).
 
@@ -520,26 +486,18 @@ Module Pipeline.
     | invalid | correct => bits_t 1
     end.
 
-  Definition Sigma (fn: custom_fn_t) : ExternalSignature :=
+  Definition Sigma (fn: ext_fn_t) : ExternalSignature :=
     match fn with
-    | Stream => {{ bits_t sz ~> unit_t ~> bits_t sz }}
-    | F => {{ bits_t sz ~> unit_t ~> bits_t sz }}
-    | G => {{ bits_t sz ~> unit_t ~> bits_t sz }}
+    | Stream => {{ bits_t sz ~> bits_t sz }}
+    | F => {{ bits_t sz ~> bits_t sz }}
+    | G => {{ bits_t sz ~> bits_t sz }}
     end.
 
-  Definition uSigma (fn: custom_fn_t) (_ _: type) : result custom_fn_t fn_tc_error := Success fn.
-  Definition iSigma idx := interop_Sigma Sigma idx.
-  Definition iuSigma := interop_uSigma uSigma.
-
   Local Notation "f [ arg ]" :=
-    (UCall (UCustomFn f) arg (UConstBits Ob))
+    (UExternalCall f arg)
       (at level 99, arg at level 99, format "f [ arg ]").
-  Local Notation "f [ arg1 ',' arg2 ]" :=
-    (UCall (UCustomFn f) arg1 arg2)
-      (at level 99, arg1 at level 99, arg2 at level 99,
-       format "f [ arg1 ','  arg2 ]").
 
-  Definition _doF : uaction _ _ _ :=
+  Definition _doF : uaction _ _ :=
     {$
        let "v" := read0(inputReg) in
        write0(inputReg,`Stream[UVar "v"]`);
@@ -552,7 +510,7 @@ Module Pipeline.
          fail
            $}.
 
-  Definition _doG : uaction _ _ _ :=
+  Definition _doG : uaction _ _ :=
     {$
     let "invalid" := read0(invalid) in
     if !"invalid" then
@@ -569,9 +527,8 @@ Module Pipeline.
       fail
         $}.
 
-
   Definition rules :=
-    tc_rules R iSigma iuSigma
+    tc_rules R Sigma
              (fun rl => match rl with
                      | doF => _doF
                      | doG => _doG
@@ -581,7 +538,7 @@ Module Pipeline.
     tc_scheduler (doG |> doF |> done).
 
   Definition circuit :=
-    compile_scheduler interop_opt (ContextEnv.(create) (readRegisters R iSigma)) rules Pipeline.
+    compile_scheduler interop_opt (ContextEnv.(create) (readRegisters R Sigma)) rules Pipeline.
 
   Definition fn_names fn :=
     match fn with
@@ -608,7 +565,7 @@ Module Pipeline.
                          | correct => "correct"
                          end;
 
-       sga_custom_fn_types := Sigma;
+       sga_ext_fn_types := Sigma;
 
        sga_rules := rules;
        sga_rule_names r := match r with
@@ -624,12 +581,12 @@ Module Pipeline.
     {| sga := sga_package;
        sp := {| sp_pkg := sga_package;
                sp_var_names := fun x => x;
-               sp_custom_fn_names := fn_names;
+               sp_ext_fn_names := fn_names;
                sp_extfuns := Some "#include ""../extfuns.hpp""
 using extfuns = pipeline_extfuns;" |};
        vp := {| vp_pkg := sga_package;
                vp_external_rules := List.nil;
-               vp_custom_fn_names := fn_names |} |}.
+               vp_ext_fn_names := fn_names |} |}.
 End Pipeline.
 
 Module RegisterFile_Ordered.
@@ -643,10 +600,9 @@ Module RegisterFile_Ordered.
   (*                        :: ("immediate", bits_t 16) *)
   (*                        :: nil |}. *)
 
-  Definition var_t := string.
   Inductive reg_t := rIndex | rData (n: Vect.index nregs) | rOutput.
-  Definition ufn_t := interop_minimal_ufn_t.
-  Inductive name_t := ReadReg.
+  Definition fn_t := empty_ext_fn_t.
+  Inductive rule_name_t := ReadReg.
 
   Definition R r :=
     match r with
@@ -655,11 +611,9 @@ Module RegisterFile_Ordered.
     | rOutput => bits_t reg_sz
     end.
 
-  Definition Sigma := interop_minimal_Sigma.
-  Definition uSigma := interop_minimal_uSigma.
+  Definition Sigma := empty_Sigma.
 
-  Definition _ReadReg : uaction _ _ interop_minimal_ufn_t :=
-
+  Definition _ReadReg : uaction _ empty_ext_fn_t :=
     {$
     let "v" := read0(rIndex) in
     write0(rIndex,"v" + `UConstBits (Bits.of_nat (log2 nregs) 1)`);
@@ -668,7 +622,7 @@ Module RegisterFile_Ordered.
   $}.
 
   Definition rules :=
-    tc_rules R iSigma iuSigma
+    tc_rules R Sigma
              (fun rl => match rl with
                      | ReadReg => _ReadReg
                      end).
@@ -695,7 +649,7 @@ Module RegisterFile_Ordered.
                          | rOutput => "rOutput"
                          end;
 
-       sga_custom_fn_types := interop_empty_Sigma;
+       sga_ext_fn_types := empty_Sigma;
 
        sga_rules := rules;
        sga_rule_names r := match r with
@@ -710,18 +664,17 @@ Module RegisterFile_Ordered.
     {| sga := sga_package;
        sp := {| sp_pkg := sga_package;
                sp_var_names := fun x => x;
-               sp_custom_fn_names := interop_empty_fn_names;
+               sp_ext_fn_names := empty_fn_names;
                sp_extfuns := None |};
        vp := {| vp_pkg := sga_package;
                vp_external_rules := List.nil;
-               vp_custom_fn_names := interop_empty_fn_names |} |}.
+               vp_ext_fn_names := empty_fn_names |} |}.
 End RegisterFile_Ordered.
 
 Module Enums.
-  Definition var_t := string.
   Inductive reg_t := rA | rB.
-  Definition ufn_t := interop_minimal_ufn_t.
-  Inductive name_t := Incr.
+  Definition fn_t := empty_ext_fn_t.
+  Inductive rule_name_t := Incr.
 
   Import ListNotations.
   Definition flag_sig :=
@@ -735,29 +688,23 @@ Module Enums.
     | rA | rB => enum_t flag_sig
     end.
 
-  Definition Sigma := interop_minimal_Sigma.
-  Definition uSigma := interop_minimal_uSigma.
+  Definition Sigma := empty_Sigma.
 
-
-  Definition _Incr : uaction _ _ interop_minimal_ufn_t :=
+  Definition _Incr : uaction _ empty_ext_fn_t :=
     {$
-       let "bits_a" := `UCall (UPrimFn (UConvFn UPack))
-                               {$read0(rA)$} (UConstBits Ob)` in
-       let "bits_b" := `UCall (UPrimFn (UConvFn UPack))
-                               {$read0(rB)$} (UConstBits Ob)` in
+       let "bits_a" := `UUnop (UConv UPack) {$read0(rA)$}` in
+       let "bits_b" := `UUnop (UConv UPack) {$read0(rB)$}` in
        let "neg_a" := !"bits_a" in
        let "succ_b" := "bits_b" + `UConstBits Ob~0~0~1` in
-       write0(rA,`UCall (UPrimFn (UConvFn (UUnpack (enum_t flag_sig))))
-                {$"neg_a"$} (UConstBits Ob)`);
-       write0(rB, `UCall (UPrimFn (UConvFn (UUnpack (enum_t flag_sig))))
-                   {$"succ_b"$} (UConstBits Ob)`)
+       write0(rA,`UUnop (UConv (UUnpack (enum_t flag_sig))) {$"neg_a"$}`);
+       write0(rB, `UUnop (UConv (UUnpack (enum_t flag_sig))) {$"succ_b"$}`)
        $}.
 
   (* Ltac __must_typecheck R Sigma tcres ::= *)
   (*   __must_typecheck_cbn R Sigma tcres. *)
 
   Definition rules :=
-    tc_rules R iSigma iuSigma
+    tc_rules R Sigma
              (fun rl => match rl with
                      | Incr => _Incr
                      end).
@@ -782,7 +729,7 @@ Module Enums.
                          | rB => "rB"
                          end;
 
-       sga_custom_fn_types := interop_empty_Sigma;
+       sga_ext_fn_types := empty_Sigma;
 
        sga_rules := rules;
        sga_rule_names r := match r with
@@ -797,18 +744,20 @@ Module Enums.
     {| sga := sga_package;
        sp := {| sp_pkg := sga_package;
                sp_var_names := fun x => x;
-               sp_custom_fn_names := interop_empty_fn_names;
+               sp_ext_fn_names := empty_fn_names;
                sp_extfuns := None |};
        vp := {| vp_pkg := sga_package;
                vp_external_rules := List.nil;
-               vp_custom_fn_names := interop_empty_fn_names |} |}.
+               vp_ext_fn_names := empty_fn_names |} |}.
 End Enums.
 
 Module IntCall.
-  Definition ufn_t := interop_minimal_ufn_t.
+  Definition fn_t := empty_ext_fn_t.
+
   Module Delay.
     Inductive reg_t := buffer.
-    Definition swap tau: UInternalFunction unit string reg_t ufn_t  :=
+
+    Definition swap tau: UInternalFunction reg_t fn_t  :=
       function "swap" ("arg1" : tau) : tau :=
       write0(buffer, "arg1");
       read0(buffer).
@@ -816,9 +765,8 @@ Module IntCall.
     Instance FiniteType_reg_t : FiniteType reg_t := _.
   End Delay.
 
-  Definition var_t := string.
   Inductive reg_t := rA | rDelay1 (d: Delay.reg_t) | rDelay2 (d: Delay.reg_t).
-  Inductive name_t := rl.
+  Inductive rule_name_t := rl.
 
   Definition R r :=
     match r with
@@ -827,27 +775,20 @@ Module IntCall.
     | rDelay2 buffer => bits_t 16
     end.
 
-  Definition Sigma := interop_minimal_Sigma.
-  Definition uSigma := interop_minimal_uSigma.
-  Notation uaction := (Syntax.uaction unit string).
+  Definition Sigma := empty_Sigma.
 
-  Definition nor (sz: nat) : UInternalFunction unit var_t reg_t ufn_t :=
+  Definition nor (sz: nat) : UInternalFunction reg_t fn_t :=
     function ("nor<" ++ string_of_nat sz ++ ">") ("arg1" : bits_t sz, "arg2" : bits_t sz) : bits_t sz :=
   !("arg1" || "arg2").
 
-  Notation UCallFn fn args :=
-    (UInternalCall (int_sig fn) (int_body fn) args).
-  Notation UCallMethod fR fSigma fn args :=
-    (UInternalCall (int_sig fn) (UCallModule fR fSigma (int_body fn)) args).
-
   Definition display :=
-    (Display.Printer (custom_fn_t := interop_empty_t) (reg_t := reg_t) (pos_t := unit)).
+    (Display.Printer (ext_fn_t := empty_ext_fn_t) (reg_t := reg_t) (pos_t := pos_t)).
 
-  Definition fSigma (fn: interop_empty_t) : ufn_t := match fn with end.
+  Definition fSigma (fn: empty_ext_fn_t) : fn_t := match fn with end.
   Definition swap8 := Delay.swap (bits_t 8).
   Definition swap16 := Delay.swap (bits_t 16).
 
-  Definition _rl : uaction string _ interop_minimal_ufn_t :=
+  Definition _rl : uaction _ empty_ext_fn_t :=
     {$
        let "a" := read0(rA) in
        let "old_a" := call rDelay2 swap16 "a" in
@@ -860,7 +801,7 @@ Module IntCall.
   (*   __must_typecheck_cbn R Sigma tcres. *)
 
   Definition rules :=
-    tc_rules R iSigma iuSigma
+    tc_rules R Sigma
              (fun rl => match rl with
                      | rl => _rl
                      end).
@@ -881,7 +822,7 @@ Module IntCall.
     end.
 
   Definition sched_result :=
-    Eval compute in interp_scheduler (ContextEnv.(create) r) interop_minimal_sigma rules sched.
+    Eval compute in interp_scheduler (ContextEnv.(create) r) empty_sigma rules sched.
 
   Definition sga_package :=
     {| sga_reg_types := R;
@@ -893,7 +834,7 @@ Module IntCall.
                          | rDelay2 buffer => "rd2_buffer"
                          end;
 
-       sga_custom_fn_types := interop_empty_Sigma;
+       sga_ext_fn_types := empty_Sigma;
 
        sga_rules := rules;
        sga_rule_names r := match r with
@@ -908,23 +849,19 @@ Module IntCall.
     {| sga := sga_package;
        sp := {| sp_pkg := sga_package;
                sp_var_names := fun x => x;
-               sp_custom_fn_names := interop_empty_fn_names;
+               sp_ext_fn_names := empty_fn_names;
                sp_extfuns := None |};
        vp := {| vp_pkg := sga_package;
                vp_external_rules := List.nil;
-               vp_custom_fn_names := interop_empty_fn_names |} |}.
+               vp_ext_fn_names := empty_fn_names |} |}.
 End IntCall.
 
 Module ExternallyCompiledRule.
   Open Scope string_scope.
-  Definition var_t := string.
-  Definition method_name_t := string.
-  Definition  custom_t:= interop_empty_t.
-  Definition ufn_t := (interop_ufn_t custom_t).
-  Definition pos_t := unit.
+  Definition fn_t := empty_ext_fn_t.
 
   Module Type Fifo.
-    Parameter  T:type.
+    Parameter T: type.
   End Fifo.
 
   Module Fifo1 (f: Fifo).
@@ -951,19 +888,15 @@ Module ExternallyCompiledRule.
       | valid0 => "valid0"
       end.
 
-
-    Local Notation uaction := (uaction pos_t method_name_t var_t reg_t ufn_t).
-
-    Definition enq : @UInternalFunction pos_t method_name_t var_t reg_t ufn_t :=
+    Definition enq : UInternalFunction reg_t fn_t :=
       function "enq" ("data" : T) : bits_t 0 :=
         if (!read0(valid0)) then
           write0(data0,"data");
-            write0(valid0,`UConstBits Ob~1`)
+          write0(valid0,`UConstBits Ob~1`)
         else
           fail.
 
-
-    Definition deq : @UInternalFunction pos_t method_name_t var_t reg_t ufn_t :=
+    Definition deq : UInternalFunction reg_t fn_t :=
       function "deq" : T :=
         if (read0(valid0)) then
           write0(valid0,`UConstBits Ob~0`);
@@ -1004,9 +937,6 @@ Module ExternallyCompiledRule.
     | Rdata => zero
     end.
 
-
-  Notation uaction := (uaction pos_t method_name_t string reg_t ufn_t).
-
   Definition _fetch :=
     {$
        let "memory" := read0(Mem) in
@@ -1024,11 +954,10 @@ Module ExternallyCompiledRule.
            $}.
 
   Definition cr := ContextEnv.(create) r.
-  Definition Sigma := interop_minimal_Sigma.
-  Definition uSigma := interop_minimal_uSigma.
+  Definition Sigma := empty_Sigma.
 
   Definition rules :=
-    tc_rules R Sigma uSigma
+    tc_rules R Sigma
              (fun rl => match rl with
                      | ding => _ding
                      | fetch => _fetch
@@ -1043,7 +972,7 @@ Module ExternallyCompiledRule.
            sga_reg_init := r;
            sga_reg_finite := _;
 
-           sga_custom_fn_types := interop_empty_Sigma;
+           sga_ext_fn_types := Sigma;
 
            sga_reg_names r := match r with
                               | Rdata => "Rdata"
@@ -1062,13 +991,12 @@ Module ExternallyCompiledRule.
   Definition sim :=
         {| sp_pkg := sga_package;
            sp_var_names := fun x => x;
-           sp_custom_fn_names := interop_empty_fn_names;
-
+           sp_ext_fn_names := empty_fn_names;
            sp_extfuns := None |}.
   Definition verilog :=
         {| vp_pkg := sga_package;
            vp_external_rules := cons fetch nil;
-           vp_custom_fn_names := interop_empty_fn_names |} .
+           vp_ext_fn_names := empty_fn_names |} .
   Definition package := {| sga := sga_package; sp := sim; vp := verilog |}.
 End ExternallyCompiledRule.
 
@@ -1076,12 +1004,7 @@ Notation zero := (Bits.zeroes _).
 
 Module GcdMachine.
   Open Scope string_scope.
-  Notation uaction := (Syntax.uaction unit string).
-  Definition var_t := string.
-  Definition method_name_t := unit.
-  Definition  custom_t:= interop_empty_t.
-  Definition ufn_t := (interop_ufn_t custom_t).
-  Definition pos_t := unit.
+  Definition fn_t := empty_ext_fn_t.
 
   Inductive reg_t := input_data |  input_valid | gcd_busy | gcd_a | gcd_b | output_data.
   Instance FiniteType_reg_t : FiniteType reg_t := _.
@@ -1113,7 +1036,7 @@ Module GcdMachine.
     | output_data => zero
     end.
 
-  Definition gcd_start : uaction string reg_t ufn_t  :=
+  Definition gcd_start : uaction reg_t fn_t  :=
     {$
        if (read0(input_valid) == `UConstBits Ob~1`
             && !read0(gcd_busy)) then
@@ -1126,23 +1049,23 @@ Module GcdMachine.
          fail
            $}.
 
-  Definition sub  : UInternalFunction unit string reg_t ufn_t :=
+  Definition sub  : UInternalFunction reg_t fn_t :=
     function "sub" ("arg1" : bits_t 16, "arg2" : bits_t 16) : bits_t 16 :=
       ("arg1" + !"arg2" + `UConstBits (Bits.of_nat 16 1)`).
 
-  Definition lt16 : UInternalFunction unit string reg_t ufn_t :=
+  Definition lt16 : UInternalFunction reg_t fn_t :=
     function "lt" ("arg1" : bits_t 16, "arg2" : bits_t 16) : bits_t 1 :=
       (funcall sub "arg1", "arg2")[`UConstBits (Bits.of_nat 4 15)`].
 
-  Fixpoint lt (sz: nat) : UInternalFunction unit var_t reg_t ufn_t :=
+  Fixpoint lt (sz: nat) : UInternalFunction reg_t fn_t :=
     match sz with
-    | O => function "lt" ("arg1" : bits_t 0, "arg2" : bits_t 0) : bits_t 0 := `UConstBits Ob~1`
+    | O => function "lt" ("arg1" : bits_t 0, "arg2" : bits_t 0) : bits_t 0 := `USugar (UConstBits Ob~1)`
     | S sz => function "lt" ("arg1" : bits_t sz, "arg2" : bits_t sz) : bits_t sz :=
       let "subLt" := funcall (lt sz) "arg1"[`UConstBits (Bits.of_nat sz 0)` :+ sz], "arg2"[`UConstBits (Bits.of_nat sz 0)` :+ sz] in
       "arg1"[`UConstBits (Bits.of_nat sz sz)`] || "arg2"[`UConstBits (Bits.of_nat sz sz)`]
     end.
 
-  Definition gcd_compute  : uaction string reg_t ufn_t  :=
+  Definition gcd_compute  : uaction reg_t fn_t  :=
     {$
        let "a" := read0(gcd_a) in
        let "b" := read0(gcd_b) in
@@ -1156,7 +1079,7 @@ Module GcdMachine.
          fail
            $}.
 
-    Definition gcd_getresult  : uaction string reg_t ufn_t  :=
+    Definition gcd_getresult  : uaction reg_t fn_t  :=
       {$
        if ( read1(gcd_a) == `UConstBits (Bits.of_nat 16 0)`
           && read1(gcd_busy)) then
@@ -1169,11 +1092,10 @@ Module GcdMachine.
   Inductive name_t := start | step_compute | get_result.
 
   Definition cr := ContextEnv.(create) init_r.
-  Definition Sigma := interop_minimal_Sigma.
-  Definition uSigma := interop_minimal_uSigma.
+  Definition Sigma := empty_Sigma.
 
   Definition rules :=
-    tc_rules R Sigma uSigma
+    tc_rules R Sigma
              (fun rl => match rl with
                      | start => gcd_start
                      | step_compute => gcd_compute
@@ -1187,7 +1109,7 @@ Module GcdMachine.
            sga_reg_init := init_r;
            sga_reg_finite := _;
 
-           sga_custom_fn_types := interop_empty_Sigma;
+           sga_ext_fn_types := empty_Sigma;
 
            sga_reg_names r := match r with
                               | input_data =>
@@ -1216,13 +1138,12 @@ Module GcdMachine.
   Definition sim :=
         {| sp_pkg := sga_package;
            sp_var_names := fun x => x;
-           sp_custom_fn_names := interop_empty_fn_names;
-
+           sp_ext_fn_names := empty_fn_names;
            sp_extfuns := None |}.
   Definition verilog :=
         {| vp_pkg := sga_package;
            vp_external_rules := nil;
-           vp_custom_fn_names := interop_empty_fn_names |} .
+           vp_ext_fn_names := empty_fn_names |} .
   Definition package := {| sga := sga_package; sp := sim; vp := verilog |}.
 End GcdMachine.
 
