Primitives.v
@@ -1,75 +1,105 @@
 Require Export SGA.Common SGA.Environments SGA.IndexUtils SGA.Types SGA.ErrorReporting.
 
-Inductive prim_display_ufn :=
-| UDisplayUtf8
-| UDisplayValue.
+Module PrimUntyped.
+  Inductive udisplay :=
+  | UDisplayUtf8
+  | UDisplayValue.
 
-Inductive prim_conv_ufn :=
-| UEq
-| UInit (tau: type)
-| UPack
-| UUnpack (tau: type)
-| UIgnore.
+  Inductive uconv :=
+  | UPack
+  | UUnpack (tau: type)
+  | UIgnore.
 
-Inductive prim_bits_ufn :=
-| USel
-| UPart (offset: nat) (width: nat)
-| UPartSubst (offset: nat) (width: nat)
-| UIndexedPart (width: nat)
-| UAnd
-| UOr
-| UNot
-| ULsl
-| ULsr
-| UConcat
-| UUIntPlus
-| UUIntLt
-| UZExtL (width: nat)
-| UZExtR (width: nat).
+  Inductive ubits1 :=
+  | UId
+  | UNot
+  | UZExtL (width: nat)
+  | UZExtR (width: nat)
+  | UPart (offset: nat) (width: nat).
 
-Inductive prim_struct_accessor :=
-| GetField
-| SubstField.
+  Inductive ubits2 :=
+  | UAnd
+  | UOr
+  | ULsl
+  | ULsr
+  | UConcat
+  | USel
+  | UPartSubst (offset: nat) (width: nat)
+  | UIndexedPart (width: nat)
+  | UUIntPlus
+  | UUIntLt.
 
-Inductive prim_struct_ufn :=
-| UDo (op: prim_struct_accessor) (f: string)
-| UDoBits (sig: struct_sig) (op: prim_struct_accessor) (f: string).
+  Inductive ustruct1 :=
+  | UGetField (f: string)
+  | UGetFieldBits (sig: struct_sig) (f: string).
 
-Inductive prim_ufn_t :=
-| UDisplayFn (fn: prim_display_ufn)
-| UConvFn (op: prim_conv_ufn)
-| UBitsFn (fn: prim_bits_ufn)
-| UStructFn (op: prim_struct_ufn).
+  Inductive ustruct2 :=
+  | USubstField (f: string)
+  | USubstFieldBits (sig: struct_sig) (f: string).
 
-Inductive prim_display_fn :=
-| DisplayUtf8 (len: nat)
-| DisplayValue (tau: type).
+  Inductive ufn1 :=
+  | UDisplay (fn: udisplay)
+  | UConv (fn: uconv)
+  | UBits1 (fn: ubits1)
+  | UStruct1 (fn: ustruct1).
 
-Inductive prim_conv_fn :=
-  Eq | Init | Pack | Unpack | Ignore.
+  Inductive ufn2 :=
+  | UEq
+  | UBits2 (fn: ubits2)
+  | UStruct2 (fn: ustruct2).
+End PrimUntyped.
 
-Inductive prim_bits_fn :=
-| Sel (sz: nat)
-| Part (sz: nat) (offset: nat) (width: nat)
-| PartSubst (sz: nat) (offset: nat) (width: nat)
-| IndexedPart (sz: nat) (width: nat)
-| And (sz: nat)
-| Or (sz: nat)
-| Not (sz: nat)
-| Lsl (bits_sz: nat) (shift_sz: nat)
-| Lsr (bits_sz: nat) (shift_sz: nat)
-| EqBits (sz: nat)
-| Concat (sz1 sz2 : nat)
-| UIntPlus (sz : nat)
-| UIntLt (sz : nat)
-| ZExtL (sz: nat) (width: nat)
-| ZExtR (sz: nat) (width: nat).
+Module PrimTyped.
+  Inductive fdisplay :=
+  | DisplayUtf8 (len: nat)
+  | DisplayValue (tau: type).
 
-Inductive prim_fn_t :=
-| DisplayFn (fn: prim_display_fn)
-| ConvFn (tau: type) (op: prim_conv_fn)
-| BitsFn (fn: prim_bits_fn)
-| StructFn (sig: struct_sig) (op: prim_struct_accessor) (f: struct_index sig).
+  Inductive fconv :=
+    Pack | Unpack | Ignore.
+
+  Inductive fbits1 :=
+  | Id (sz: nat)
+  | Not (sz: nat)
+  | ZExtL (sz: nat) (width: nat)
+  | ZExtR (sz: nat) (width: nat)
+  | Part (sz: nat) (offset: nat) (width: nat).
+
+  Inductive fbits2 :=
+  | And (sz: nat)
+  | Or (sz: nat)
+  | Lsl (bits_sz: nat) (shift_sz: nat)
+  | Lsr (bits_sz: nat) (shift_sz: nat)
+  | EqBits (sz: nat)
+  | Concat (sz1 sz2 : nat)
+  | Sel (sz: nat)
+  | PartSubst (sz: nat) (offset: nat) (width: nat)
+  | IndexedPart (sz: nat) (width: nat)
+  | UIntPlus (sz : nat)
+  | UIntLt (sz: nat).
+
+  Inductive fstruct1 :=
+  | GetField.
+
+  Inductive fstruct2 :=
+  | SubstField.
+
+  Inductive fn1 :=
+  | Display (fn: fdisplay)
+  | Conv (tau: type) (fn: fconv)
+  | Bits1 (fn: fbits1)
+  | Struct1 (fn: fstruct1) (sig: struct_sig) (f: struct_index sig).
+
+  Inductive fn2 :=
+  | Eq (tau: type)
+  | Bits2 (fn: fbits2)
+  | Struct2 (fn: fstruct2) (sig: struct_sig) (f: struct_index sig).
+
+  Definition GetFieldBits (sig: struct_sig) (idx: struct_index sig) : fbits1 :=
+    Part (struct_sz sig) (field_offset_right sig idx) (field_sz sig idx).
+
+  Definition SubstFieldBits (sig: struct_sig) (idx: struct_index sig) : fbits2 :=
+    PartSubst (struct_sz sig) (field_offset_right sig idx) (field_sz sig idx).
+End PrimTyped.
 
 (* Like Nat.log2_iter, but switches to next power of two one number earlier
    (computes ceil(log2(n)) instead of floor(log2(n))). *)
@@ -85,214 +115,260 @@ Fixpoint log2_iter k_fuel p_logn q_n r_buffer :=
 
 Definition log2 n := log2_iter (pred n) 0 1 0.
 
-Definition GetFieldBits (sig: struct_sig) (idx: struct_index sig) : prim_fn_t :=
-  BitsFn (Part (struct_sz sig) (field_offset_right sig idx) (field_sz sig idx)).
+Module PrimTypeInference.
+  Import PrimUntyped PrimTyped.
 
-Definition SubstFieldBits (sig: struct_sig) (idx: struct_index sig) : prim_fn_t :=
-  BitsFn (PartSubst (struct_sz sig) (field_offset_right sig idx) (field_sz sig idx)).
+  Definition find_field sig f : result _ fn_tc_error :=
+    opt_result (List_assoc f sig.(struct_fields)) (Arg1, UnboundField f sig).
 
-Definition prim_uSigma (fn: prim_ufn_t) (tau1 tau2: type): result prim_fn_t fn_tc_error :=
-  match fn with
-  | UDisplayFn fn =>
+  Definition tc1 (fn: ufn1) (tau1: type): result fn1 fn_tc_error :=
     match fn with
-    | UDisplayUtf8 =>
+    | UDisplay fn =>
+      match fn with
+      | UDisplayUtf8 =>
+        let/res sz1 := assert_bits_t Arg1 tau1 in
+        Success (Display (DisplayUtf8 sz1))
+      | UDisplayValue =>
+        Success (Display (DisplayValue tau1))
+      end
+    | UConv fn =>
+      Success (match fn with
+               | UPack => Conv tau1 Pack
+               | UUnpack tau => Conv tau Unpack
+               | UIgnore => Conv tau1 Ignore
+               end)
+    | UBits1 fn =>
       let/res sz1 := assert_bits_t Arg1 tau1 in
-      Success (DisplayFn (DisplayUtf8 sz1))
-    | UDisplayValue =>
-      Success (DisplayFn (DisplayValue tau1))
-    end
-  | UConvFn op =>
-    Success (match op with
-             | UEq => ConvFn tau1 Eq
-             | UPack => ConvFn tau1 Pack
-             | UInit tau => ConvFn tau Init
-             | UUnpack tau => ConvFn tau Unpack
-             | UIgnore => ConvFn tau1 Ignore
-             end)
-  | UBitsFn fn =>
-    let/res sz1 := assert_bits_t Arg1 tau1 in
-    let/res sz2 := assert_bits_t Arg2 tau2 in
-    Success (BitsFn match fn with
-                    | USel => Sel sz1
-                    | UPart offset width => Part sz1 offset width
-                    | UPartSubst offset width => PartSubst sz1 offset width
-                    | UIndexedPart width => IndexedPart sz1 width
-                    | UAnd => And sz1
-                    | UOr => Or sz1
-                    | UNot => Not sz1
-                    | ULsl => Lsl sz1 sz2
-                    | ULsr => Lsr sz1 sz2
-                    | UConcat => Concat sz1 sz2
-                    | UUIntPlus => UIntPlus sz1
-                    | UUIntLt => UIntLt sz1
-                    | UZExtL width => ZExtL sz1 width
-                    | UZExtR width => ZExtR sz1 width
-                    end)
-  | UStructFn fn =>
-    let find_field sig f :=
-        opt_result (List_assoc f sig.(struct_fields)) (Arg1, UnboundField f sig) in
-    match fn with
-      | UDo op f =>
+      Success (Bits1 match fn with
+                     | UId => Id sz1
+                     | UNot => Not sz1
+                     | UZExtL width => ZExtL sz1 width
+                     | UZExtR width => ZExtR sz1 width
+                     | UPart offset width => Part sz1 offset width
+                     end)
+    | UStruct1 fn =>
+      match fn with
+      | UGetField f =>
         let/res sig := assert_struct_t Arg1 tau1 in
         let/res idx := find_field sig f in
-        Success (StructFn sig op idx)
-      | UDoBits sig op f =>
+        Success (Struct1 GetField sig idx)
+      | UGetFieldBits sig f =>
         let/res idx := find_field sig f in
-        Success match op with
-                | GetField => GetFieldBits sig idx
-                | SubstField => SubstFieldBits sig idx
-                end
-    end
-  end.
+        Success (Bits1 (GetFieldBits sig idx))
+      end
+    end.
 
-Definition prim_Sigma (fn: prim_fn_t) : ExternalSignature :=
-  match fn with
-  | DisplayFn fn =>
+  Definition tc2 (fn: ufn2) (tau1: type) (tau2: type): result fn2 fn_tc_error :=
     match fn with
-    | DisplayUtf8 sz => {{ bits_t sz ~> unit_t ~> unit_t }}
-    | DisplayValue tau => {{ tau ~> unit_t ~> unit_t }}
-    end
-  | ConvFn tau op =>
-    match op with
-    | Eq => {{ tau ~> tau ~> bits_t 1 }}
-    | Init => {{ unit_t ~> unit_t ~> tau }}
-    | Pack => {{ tau ~> unit_t ~> bits_t (type_sz tau) }}
-    | Unpack => {{ bits_t (type_sz tau) ~> unit_t ~> tau }}
-    | Ignore => {{ tau ~> unit_t ~> unit_t }}
-    end
-  | BitsFn fn =>
+    | UEq => Success (Eq tau1)
+    | UBits2 fn =>
+      let/res sz1 := assert_bits_t Arg1 tau1 in
+      let/res sz2 := assert_bits_t Arg2 tau2 in
+      Success (Bits2 match fn with
+                     | USel => Sel sz1
+                     | UPartSubst offset width => PartSubst sz1 offset width
+                     | UIndexedPart width => IndexedPart sz1 width
+                     | UAnd => And sz1
+                     | UOr => Or sz1
+                     | ULsl => Lsl sz1 sz2
+                     | ULsr => Lsr sz1 sz2
+                     | UConcat => Concat sz1 sz2
+                     | UUIntPlus => UIntPlus sz1
+                     | UUIntLt => UIntLt sz1
+                     end)
+    | UStruct2 fn =>
+      match fn with
+      | USubstField f =>
+        let/res sig := assert_struct_t Arg1 tau1 in
+        let/res idx := find_field sig f in
+        Success (Struct2 SubstField sig idx)
+      | USubstFieldBits sig f =>
+        let/res idx := find_field sig f in
+        Success (Bits2 (SubstFieldBits sig idx))
+      end
+    end.
+End PrimTypeInference.
+
+Module CircuitSignatures.
+  Import PrimTyped.
+  Import CSigNotations.
+
+  Definition CSigma1 (fn: fbits1) : CSig 1 :=
     match fn with
-    | Sel sz => {{ bits_t sz ~> bits_t (log2 sz) ~> bits_t 1 }}
-    | Part sz offset width => {{ bits_t sz ~> unit_t ~> bits_t width }}
-    | PartSubst sz offset width => {{ bits_t sz ~> bits_t width ~> bits_t sz }}
-    | IndexedPart sz width => {{ bits_t sz ~> bits_t (log2 sz) ~> bits_t width }}
-    | And sz => {{ bits_t sz ~> bits_t sz ~> bits_t sz }}
-    | Or sz => {{ bits_t sz ~> bits_t sz ~> bits_t sz }}
-    | Not sz => {{ bits_t sz ~> unit_t ~> bits_t sz }}
-    | Lsl bits_sz shift_sz => {{ bits_t bits_sz ~> bits_t shift_sz ~> bits_t bits_sz }}
-    | Lsr bits_sz shift_sz => {{ bits_t bits_sz ~> bits_t shift_sz ~> bits_t bits_sz }}
-    | EqBits sz => {{ bits_t sz ~> bits_t sz ~> bits_t 1 }}
-    | Concat sz1 sz2 => {{ bits_t sz1 ~> bits_t sz2 ~> bits_t (sz2 + sz1) }}
-    | UIntPlus sz => {{ bits_t sz ~> bits_t sz ~> bits_t sz }}
-    | UIntLt sz => {{ bits_t sz ~> bits_t sz ~> bits_t 1 }}
-    | ZExtL sz width => {{ bits_t sz ~> unit_t ~> bits_t (Nat.max sz width) }}
-    | ZExtR sz width => {{ bits_t sz ~> unit_t ~> bits_t (Nat.max sz width) }}
-    end
-  | @StructFn sig op idx =>
-    match op with
-    | GetField => {{ struct_t sig ~> unit_t ~> field_type sig idx }}
-    | SubstField => {{ struct_t sig ~> field_type sig idx ~> struct_t sig }}
-    end
-  end.
+    | Id sz => {{ sz ~> sz }}
+    | Not sz => {{ sz ~> sz }}
+    | ZExtL sz width => {{ sz ~> (Nat.max sz width) }}
+    | ZExtR sz width => {{ sz ~> (Nat.max sz width) }}
+    | Part sz offset width => {{ sz ~> width }}
+    end.
 
-Definition prim_sel {sz} (bs: bits sz) (idx: bits (log2 sz)) :=
-  match Bits.to_index sz idx with
-  | Some idx => Bits.nth bs idx
-  | _ => false (* TODO: x *)
-  end.
-
-Definition prim_uint_plus {sz} (bs1 bs2: bits sz) :=
-  Bits.of_N sz (Bits.to_N bs1 + Bits.to_N bs2)%N.
-
-Definition prim_uint_lt {sz} (bs1 bs2: bits sz) :=
-  Ob~(Bits.to_N bs1 <? Bits.to_N bs2)%N.
-
-(* Fixpoint type_accessor (tau: type) : Type := *)
-(*   match tau with *)
-(*   | bits_t _sz => unit *)
-(*   | struct_t fields => *)
-(*     let fs := fields.(struct_fields) in *)
-(*     let field_accessors := List.map (fun '(k, tau) => type_accessor tau) fs in *)
-(*     { k: index (List.length field_accessors) & List_nth field_accessors k } *)
-(*   end. *)
-
-Definition prim_part {sz} (bs: bits sz) (offset: nat) (width: nat) :=
-  vect_extend_end_firstn (vect_firstn width (vect_skipn offset bs)) false.
-
-Lemma prim_part_subst_cast :
-  forall sz width offset,
-    Nat.min sz (Nat.min offset sz + (width + (sz - (offset + width)))) = sz.
-Proof.
-  induction sz, width, offset; cbn; auto using Min.min_idempotent.
-  - f_equal; apply (IHsz 0 offset).
-  - f_equal; apply (IHsz width 0).
-  - f_equal; apply (IHsz (S width) offset).
-Defined.
-
-Definition prim_part_subst {sz}
-           (bs: bits sz)
-           (offset: nat)
-           (width: nat)
-           (v: bits width) : bits sz :=
-  let head := vect_firstn offset bs in
-  let tail := vect_skipn (offset + width) bs in
-  ltac:(rewrite <- (prim_part_subst_cast sz width offset);
-          exact (vect_firstn sz (vect_app head (vect_app v tail)))).
-
-(* destruct offset. *)
-(* - destruct width. *)
-(*   + exact bs. *)
-(*   + *)
-(* destruct sz. *)
-(* - exact vect_nil. *)
-(* - destruct width. *)
-(*   destruct offset. *)
-(*   + destruct width. *)
-
-Fixpoint get_field fields
-         (v: struct_denote fields)
-         (idx: index (List.length fields))
-         {struct fields}
-  : type_denote (snd (List_nth fields idx)).
-  destruct fields, idx, p; cbn.
-  - apply (fst v).
-  - apply (get_field fields (snd v) a).
-Defined.
-
-Fixpoint subst_field fields
-         (v: struct_denote fields)
-         (idx: index (List.length fields))
-         (v': type_denote (snd (List_nth fields idx)))
-         {struct fields}
-  : (struct_denote fields).
-  destruct fields, idx, p; cbn.
-  - apply (v', snd v).
-  - apply (fst v, subst_field fields (snd v) a v').
-Defined.
-
-Definition prim_sigma (fn: prim_fn_t) : prim_Sigma fn :=
-  match fn with
-  | DisplayFn fn =>
+  Definition CSigma2 (fn: PrimTyped.fbits2) : CSig 2 :=
     match fn with
-    | DisplayUtf8 _ => fun _ _ => Ob
-    | DisplayValue _ => fun _ _ => Ob
-    end
-  | ConvFn tau fn =>
+    | Sel sz => {{ sz ~> (log2 sz) ~> 1 }}
+    | PartSubst sz offset width => {{ sz ~> width ~> sz }}
+    | IndexedPart sz width => {{ sz ~> (log2 sz) ~> width }}
+    | And sz => {{ sz ~> sz ~> sz }}
+    | Or sz => {{ sz ~> sz ~> sz }}
+    | Lsl bits_sz shift_sz => {{ bits_sz ~> shift_sz ~> bits_sz }}
+    | Lsr bits_sz shift_sz => {{ bits_sz ~> shift_sz ~> bits_sz }}
+    | EqBits sz => {{ sz ~> sz ~> 1 }}
+    | Concat sz1 sz2 => {{ sz1 ~> sz2 ~> (sz2 + sz1) }}
+    | UIntPlus sz => {{ sz ~> sz ~> sz }}
+    | UIntLt sz => {{ sz ~> sz ~> 1 }}
+    end.
+End CircuitSignatures.
+
+Module PrimSignatures.
+  Import PrimUntyped PrimTyped CircuitSignatures.
+  Import SigNotations.
+
+  Definition Sigma1 (fn: fn1) : Sig 1 :=
     match fn with
-    | Eq => fun v1 v2 => if eq_dec v1 v2 then Ob~1 else Ob~0
-    | Init => fun _ _ => value_of_bits (Bits.zeroes (type_sz tau))
-    | Pack => fun v _ => bits_of_value v
-    | Unpack => fun bs _ => value_of_bits bs
-    | Ignore => fun _ _ => Ob
-    end
-  | BitsFn fn =>
+    | Conv tau fn =>
+      match fn with
+      | Pack => {{ tau ~> bits_t (type_sz tau) }}
+      | Unpack => {{ bits_t (type_sz tau) ~> tau }}
+      | Ignore => {{ tau ~> unit_t }}
+      end
+    | Display fn =>
+      {{ match fn with
+         | DisplayUtf8 sz => bits_t sz
+         | DisplayValue tau => tau
+         end ~> unit_t }}
+    | Bits1 fn => Sig_of_CSig (CSigma1 fn)
+    | Struct1 GetField sig idx => {{ struct_t sig ~> field_type sig idx }}
+    end.
+
+  Definition Sigma2 (fn: fn2) : Sig 2 :=
     match fn with
-    | Sel _ => fun bs idx => Ob~(prim_sel bs idx)
-    | Part _ offset width => fun bs _ => prim_part bs offset width
-    | PartSubst _ offset width => fun bs repl => prim_part_subst bs offset width repl
-    | IndexedPart _ width => fun bs offset => prim_part bs (Bits.to_nat offset) width
+    | Eq tau => {{ tau ~> tau ~> bits_t 1 }}
+    | Struct2 SubstField sig idx => {{ struct_t sig ~> field_type sig idx ~> struct_t sig }}
+    | Bits2 fn => Sig_of_CSig (CSigma2 fn)
+    end.
+End PrimSignatures.
+
+Module BitFuns.
+  Definition sel {sz} (bs: bits sz) (idx: bits (log2 sz)) :=
+    Ob~match Bits.to_index sz idx with
+       | Some idx => Bits.nth bs idx
+       | _ => false (* TODO: x *)
+       end.
+
+  Definition lsl {bits_sz shift_sz} (bs: bits bits_sz) (places: bits shift_sz) :=
+    Bits.lsl (Bits.to_nat places) bs.
+
+  Definition lsr {bits_sz shift_sz} (bs: bits bits_sz) (places: bits shift_sz) :=
+    Bits.lsr (Bits.to_nat places) bs.
+
+  Definition eq_bits {sz} (bs1 bs2: bits sz) :=
+    if eq_dec bs1 bs2 then Ob~1 else Ob~0.
+
+  Definition concat {sz1 sz2} (bs1: bits sz1) (bs2: bits sz2) :=
+    Bits.app bs1 bs2.
+
+  Definition uint_plus {sz} (bs1 bs2: bits sz) :=
+    Bits.of_N sz (Bits.to_N bs1 + Bits.to_N bs2)%N.
+
+  Definition uint_lt {sz} (bs1 bs2: bits sz) :=
+    Ob~(Bits.to_N bs1 <? Bits.to_N bs2)%N.
+
+  Definition part {sz} (offset: nat) (width: nat) (bs: bits sz) :=
+    vect_extend_end_firstn (vect_firstn width (vect_skipn offset bs)) false.
+
+  Lemma part_subst_cast :
+    forall sz width offset,
+      Nat.min sz (Nat.min offset sz + (width + (sz - (offset + width)))) = sz.
+  Proof.
+    induction sz, width, offset; cbn; auto using Min.min_idempotent.
+    - f_equal; apply (IHsz 0 offset).
+    - f_equal; apply (IHsz width 0).
+    - f_equal; apply (IHsz (S width) offset).
+  Defined.
+
+  Definition part_subst {sz}
+             (offset: nat)
+             (width: nat)
+             (bs: bits sz)
+             (v: bits width) : bits sz :=
+    let head := vect_firstn offset bs in
+    let tail := vect_skipn (offset + width) bs in
+    ltac:(rewrite <- (part_subst_cast sz width offset);
+            exact (vect_firstn sz (vect_app head (vect_app v tail)))).
+
+  Fixpoint get_field fields
+           (v: struct_denote fields)
+           (idx: index (List.length fields))
+           {struct fields}
+    : type_denote (snd (List_nth fields idx)).
+    destruct fields, idx, p; cbn.
+    - apply (fst v).
+    - apply (get_field fields (snd v) a).
+  Defined.
+
+  Fixpoint subst_field fields
+           (v: struct_denote fields)
+           (idx: index (List.length fields))
+           (v': type_denote (snd (List_nth fields idx)))
+           {struct fields}
+    : (struct_denote fields).
+    destruct fields, idx, p; cbn.
+    - apply (v', snd v).
+    - apply (fst v, subst_field fields (snd v) a v').
+  Defined.
+End BitFuns.
+
+Module CircuitPrimSpecs.
+  Import PrimTyped BitFuns.
+
+  Definition sigma1 (fn: PrimTyped.fbits1) : CSig_denote (CircuitSignatures.CSigma1 fn) :=
+    match fn with
+    | Id _ => fun bs => bs
+    | Not _ => fun bs => Bits.map negb bs
+    | ZExtL sz width => fun bs => Bits.extend_end bs width false
+    | ZExtR sz width => fun bs => Bits.extend_beginning bs width false
+    | Part _ offset width => part offset width
+    end.
+
+  Definition sigma2 (fn: PrimTyped.fbits2) : CSig_denote (CircuitSignatures.CSigma2 fn) :=
+    match fn with
+    | Sel _ => sel
+    | PartSubst _ offset width => part_subst offset width
+    | IndexedPart _ width => fun bs offset => part (Bits.to_nat offset) width bs
     | And _ => Bits.map2 andb
     | Or _ => Bits.map2 orb
-    | Not _ => fun bs _ => Bits.map negb bs
-    | Lsl _ _ => fun bs places => Bits.lsl (Bits.to_nat places) bs
-    | Lsr _ _ => fun bs places => Bits.lsr (Bits.to_nat places) bs
-    | EqBits sz => fun bs1 bs2 => if eq_dec bs1 bs2 then Ob~1 else Ob~0
-    | UIntPlus _ => fun bs1 bs2 => prim_uint_plus bs1 bs2
-    | UIntLt _ => fun bs1 bs2 => prim_uint_lt bs1 bs2
-    | Concat _ _ => fun bs1 bs2 => Bits.app bs1 bs2
-    | ZExtL sz width => fun bs _ => Bits.extend_end bs width false
-    | ZExtR sz width => fun bs _ => Bits.extend_beginning bs width false
-    end
-  | StructFn sig GetField idx => fun s _ => get_field sig.(struct_fields) s idx
-  | StructFn sig SubstField idx => fun s v => subst_field sig.(struct_fields) s idx v
-  end.
+    | Lsl _ _ => lsl
+    | Lsr _ _ => lsr
+    | EqBits sz => eq_bits
+    | Concat _ _ => concat
+    | UIntPlus _ => uint_plus
+    | UIntLt _ => uint_lt
+    end.
+End CircuitPrimSpecs.
+
+Module PrimSpecs.
+  Import PrimTyped BitFuns.
+
+  Definition sigma1 (fn: fn1) : Sig_denote (PrimSignatures.Sigma1 fn) :=
+    match fn with
+    | Display fn =>
+      match fn with
+      | DisplayUtf8 _ => fun _ => Ob
+      | DisplayValue tau => fun _ => Ob
+      end
+    | Conv tau fn =>
+      match fn with
+      | Pack => fun v => bits_of_value v
+      | Unpack => fun bs => value_of_bits bs
+      | Ignore => fun _ => Ob
+      end
+    | Bits1 fn => CircuitPrimSpecs.sigma1 fn
+    | Struct1 GetField sig idx => fun s => get_field sig.(struct_fields) s idx
+    end.
+
+  Definition sigma2 (fn: fn2) : Sig_denote (PrimSignatures.Sigma2 fn) :=
+    match fn with
+    | Eq tau => fun v1 v2 => if eq_dec v1 v2 then Ob~1 else Ob~0
+    | Bits2 fn => CircuitPrimSpecs.sigma2 fn
+    | Struct2 SubstField sig idx => fun s v => subst_field sig.(struct_fields) s idx v
+    end.
+End PrimSpecs.
