TypeInference.v
@@ -6,26 +6,30 @@ Require Import Coq.Lists.List.
 Import ListNotations.
 
 Section ErrorReporting.
-  Context {pos_t fn_name_t var_t reg_t fn_t: Type}.
+  Context {pos_t var_t fn_name_t reg_t ext_fn_t: Type}.
   Context {R: reg_t -> type}
-          {Sigma: fn_t -> ExternalSignature}.
+          {Sigma: ext_fn_t -> ExternalSignature}.
 
   Definition lift_basic_error_message
              (pos: pos_t) {sig tau} (e: action var_t R Sigma sig tau)
              (err: basic_error_message) : error pos_t var_t fn_name_t :=
     {| epos := pos;
-       emsg := BasicError match err with
-                          | TypeMismatch _ actual expected => TypeMismatch e actual expected
-                          | KindMismatch _ actual expected => KindMismatch e actual expected
-                          | _ => err
-                          end |}.
+       emsg := BasicError err;
+       esource := ErrSrc e |}.
 
-  Definition lift_fn_tc_result
+  Definition lift_fn1_tc_result
+             {A sig tau}
+             pos (e: action var_t R Sigma sig tau)
+             (r: result A fn_tc_error)
+    : result A (error pos_t var_t fn_name_t) :=
+    result_map_failure (fun '(side, err) => lift_basic_error_message pos e err) r.
+
+  Definition lift_fn2_tc_result
              {A sig1 tau1 sig2 tau2}
              pos1 (e1: action var_t R Sigma sig1 tau1)
              pos2 (e2: action var_t R Sigma sig2 tau2)
              (r: result A fn_tc_error)
-    : (result A (error pos_t var_t fn_name_t)) :=
+    : result A (error pos_t var_t fn_name_t) :=
     result_map_failure (fun '(side, err) =>
                           match side with
                           | Arg1 => lift_basic_error_message pos1 e1 err
@@ -34,29 +38,27 @@ Section ErrorReporting.
 End ErrorReporting.
 
 Section TypeInference.
-  Context {pos_t rule_name_t fn_name_t var_t reg_t ufn_t fn_t: Type}.
+  Context {pos_t rule_name_t fn_name_t var_t reg_t ext_fn_t: Type}.
   Context {var_t_eq_dec: EqDec var_t}.
 
   Context (R: reg_t -> type).
-  Context (Sigma: fn_t -> ExternalSignature).
-  Context (uSigma: forall (fn: ufn_t) (tau1 tau2: type), result fn_t fn_tc_error).
+  Context (Sigma: ext_fn_t -> ExternalSignature).
 
-  Notation usugar := (usugar pos_t fn_name_t var_t).
-  Notation uaction := (uaction pos_t fn_name_t var_t).
+  Notation usugar := (usugar pos_t var_t fn_name_t).
+  Notation uaction := (uaction pos_t var_t fn_name_t).
   Notation uscheduler := (uscheduler pos_t rule_name_t).
 
   Notation action := (action var_t R Sigma).
   Notation rule := (rule var_t R Sigma).
   Notation scheduler := (scheduler rule_name_t).
-  Notation schedule := (schedule rule_name_t var_t R Sigma).
 
   Section Action.
     Notation error := (error pos_t var_t fn_name_t).
     Notation error_message := (error_message var_t fn_name_t).
     Notation result A := (result A error).
 
-    Definition mkerror pos msg : error :=
-      {| epos := pos; emsg := msg |}.
+    Definition mkerror {T} pos msg (src: T) : error :=
+      {| epos := pos; emsg := msg; esource := ErrSrc src |}.
 
     Notation "` x" := (projT1 x) (at level 0).
     Notation "`` x" := (projT2 x) (at level 0).
@@ -67,57 +69,59 @@ Section TypeInference.
     Proof.
       destruct (eq_dec tau1 tau2); subst.
       - exact (Success e).
-      - exact (Failure {| epos := pos; emsg := emsg |}).
+      - exact (Failure (mkerror pos emsg e)).
     Defined.
 
     Definition cast_action pos {sig tau1} tau2 (e: action sig tau1) :=
-      cast_action' pos tau2 e (BasicError (TypeMismatch e tau1 tau2)).
+      cast_action' pos tau2 e (BasicError (TypeMismatch tau1 tau2)).
 
     Definition cast_rule (pos: pos_t) {tau} (e: action [] tau) :=
       cast_action' pos (bits_t 0) e (IncorrectRuleType tau).
 
     Notation EX Px := (existT _ _ Px).
 
-    Fixpoint actpos {reg_t ufn_t} pos (e: uaction reg_t ufn_t) :=
+    Fixpoint actpos {reg_t ext_fn_t} pos (e: uaction reg_t ext_fn_t) :=
       match e with
       | UAPos p _ => p
       | _ => pos
       end.
 
-    Fixpoint assert_argtypes' {sig} nexpected (fn_name: fn_name_t) pos
+    Fixpoint assert_argtypes' {T} {sig} (src: T) nexpected (fn_name: fn_name_t) pos
              (args_desc: tsig var_t)
              (args: list (pos_t * {tau : type & action sig tau}))
       : result (context (K := (var_t * type)) (fun '(_, tau) => action sig tau) args_desc) :=
       match args_desc, args with
       | [], [] => Success CtxEmpty
-      | [], _ => Failure (mkerror pos (TooManyArguments fn_name nexpected (List.length args)))
-      | _, [] => Failure (mkerror pos (TooFewArguments fn_name nexpected (List.length args_desc)))
+      | [], _ => Failure (mkerror pos (TooManyArguments fn_name nexpected (List.length args)) src)
+      | _, [] => Failure (mkerror pos (TooFewArguments fn_name nexpected (List.length args_desc)) src)
       | (name1, tau1) :: fn_sig, (pos1, arg1) :: args =>
         let/res arg1 := cast_action pos1 tau1 ``arg1  in
-        let/res ctx := assert_argtypes' nexpected fn_name pos fn_sig args in
+        let/res ctx := assert_argtypes' src nexpected fn_name pos fn_sig args in
         Success (CtxCons (name1, tau1) arg1 ctx)
       end.
 
-    Definition assert_argtypes {sig} (fn_name: fn_name_t) pos
-             (args_desc: tsig var_t)
-             (args: list (pos_t * {tau : type & action sig tau}))
+    Definition assert_argtypes {T} {sig}
+               (src: T)
+               (fn_name: fn_name_t) pos
+               (args_desc: tsig var_t)
+               (args: list (pos_t * {tau : type & action sig tau}))
       : result (context (K := (var_t * type)) (fun '(_, tau) => action sig tau) args_desc) :=
-      assert_argtypes' (List.length args_desc) fn_name pos args_desc args.
+      assert_argtypes' src (List.length args_desc) fn_name pos args_desc args.
 
     Fixpoint type_action
              (pos: pos_t) (sig: tsig var_t)
-             (e: uaction reg_t ufn_t) {struct e}
+             (e: uaction reg_t ext_fn_t) {struct e}
       : result ({ tau: type & action sig tau }) :=
       match e with
       | UError err => Failure err
-      | USugar _ => Failure (mkerror pos SugaredConstructorInAst)
+      | USugar _ => Failure (mkerror pos SugaredConstructorInAst e)
       | UFail n => Success (EX (Fail (bits_t n)))
       | UVar var =>
-        let/res tau_m := opt_result (assoc var sig) (mkerror pos (UnboundVariable var)) in
+        let/res tau_m := opt_result (assoc var sig) (mkerror pos (UnboundVariable var) e) in
         Success (EX (Var ``tau_m))
       | UConst cst => Success (EX (Const cst))
       | UAssign var ex =>
-        let/res tau_m := opt_result (assoc var sig) (mkerror pos (UnboundVariable var)) in
+        let/res tau_m := opt_result (assoc var sig) (mkerror pos (UnboundVariable var) e) in
         let/res ex' := type_action pos sig ex in
         let/res ex' := cast_action (actpos pos ex) `tau_m (``ex') in
         Success (EX (Assign (k := var) (tau := `tau_m) ``tau_m ex'))
@@ -142,27 +146,38 @@ Section TypeInference.
         let/res value' := type_action pos sig value in
         let/res value' := cast_action (actpos pos value) (R idx) (``value') in
         Success (EX (Write port idx value'))
-      | UInternalCall fn_sig fn_body args =>
+      | UInternalCall fn args =>
         let/res tc_args := result_list_map (type_action pos sig) args in
         let arg_positions := List.map (actpos pos) args in
         let tc_args_w_pos := List.combine arg_positions tc_args in
-        let/res arg_ctx := assert_argtypes fn_sig.(int_name) pos fn_sig.(int_args) tc_args_w_pos in
-        let/res fn_body' := type_action (actpos pos fn_body) fn_sig.(int_args) fn_body in
-        let/res fn_body' := cast_action (actpos pos fn_body) fn_sig.(int_retType) (``fn_body') in
-        Success (EX (InternalCall sig fn_sig.(int_args) fn_body' arg_ctx))
-      | UCall ufn arg1 arg2 =>
+        let/res arg_ctx := assert_argtypes e fn.(int_name) pos fn.(int_argspec) tc_args_w_pos in
+        let/res fn_body' := type_action (actpos pos fn.(int_body)) fn.(int_argspec) fn.(int_body) in
+        let/res fn_body' := cast_action (actpos pos fn.(int_body)) fn.(int_retType) (``fn_body') in
+        Success (EX (InternalCall sig fn.(int_argspec) fn_body' arg_ctx))
+      | UUnop fn arg1 =>
+        let pos1 := actpos pos arg1 in
         let/res arg1' := type_action pos sig arg1 in
-        let/res arg2' := type_action pos sig arg2 in
+        let/res fn := lift_fn1_tc_result pos1 ``arg1' (PrimTypeInference.tc1 fn `arg1') in
+        let/res arg1' := cast_action pos1 (PrimSignatures.Sigma1 fn).(arg1Type) (``arg1') in
+        Success (EX (Unop fn arg1'))
+      | UBinop fn arg1 arg2 =>
         let pos1 := actpos pos arg1 in
         let pos2 := actpos pos arg2 in
-        let/res fn := lift_fn_tc_result pos1 ``arg1' pos2 ``arg2' (uSigma ufn `arg1' `arg2') in
+        let/res arg1' := type_action pos sig arg1 in
+        let/res arg2' := type_action pos sig arg2 in
+        let/res fn := lift_fn2_tc_result pos1 ``arg1' pos2 ``arg2' (PrimTypeInference.tc2 fn `arg1' `arg2') in
+        let/res arg1' := cast_action pos1 (PrimSignatures.Sigma2 fn).(arg1Type) (``arg1') in
+        let/res arg2' := cast_action pos2 (PrimSignatures.Sigma2 fn).(arg2Type) (``arg2') in
+        Success (EX (Binop fn arg1' arg2'))
+      | UExternalCall fn arg1 =>
+        let pos1 := actpos pos arg1 in
+        let/res arg1' := type_action pos1 sig arg1 in
         let/res arg1' := cast_action pos1 (Sigma fn).(arg1Type) (``arg1') in
-        let/res arg2' := cast_action pos2 (Sigma fn).(arg2Type) (``arg2') in
-        Success (EX (Call fn arg1' arg2'))
+        Success (EX (ExternalCall fn arg1'))
       | UAPos pos e => type_action pos sig e
       end.
 
-    Definition type_rule (pos: pos_t) (e: uaction reg_t ufn_t) : result rule :=
+    Definition type_rule (pos: pos_t) (e: uaction reg_t ext_fn_t) : result rule :=
       let/res rl := type_action pos [] e in
       cast_rule pos (``rl).
   End Action.
